Question for Bryan on preconditions

src/crypto/loopunroll/loopunroll.s.dfy
@@ -3,10 +3,58 @@ include "../../lib/util/operations.s.dfy"
 include "../../lib/util/words_and_bytes.s.dfy"
 include "../../lib/collections/Seqs.s.dfy"
 include "../../arch/x64/def.s.dfy"
+include "../../arch/x64/vale.i.dfy"
+include "../../lib/util/dafny_wrappers.i.dfy"
 
 module LoopUnrollModule {
 
 import opened x64_def_s
 import opened types_s
+import opened x64_vale_i
+import opened dafny_wrappers_i
+
+lemma lemma_BitwiseAdd64()
+    ensures  forall x:uint64, y:uint64 :: x + y < 0x1_0000_0000_0000_0000 ==> BitwiseAdd64(x, y) == x + y
+    ensures  forall x:uint64, y:uint64 :: x + y >= 0x1_0000_0000_0000_0000 ==> BitwiseAdd64(x, y) == x + y - 0x1_0000_0000_0000_0000
+    ensures  forall x:uint64 :: BitwiseAdd64(x, 0) == x;
+{
+    reveal_BitwiseAdd64();
+}
+
+predicate ValidDstAddr64(h:Heaplets, id:heaplet_id, addr:int)
+{
+  id in h  && h[id].Heaplet64?   && addr in h[id].mem64
+}
+
+predicate ValidSrcAddr64(h:Heaplets, id:heaplet_id, addr:int, taint:taint) 
+{
+ id in h  && h[id].Heaplet64?   && addr in h[id].mem64 && h[id].mem64[addr].t == taint
+}
+
+lemma lemma_ValidDstAddr64(mem:Heaplets, id:heaplet_id, addr : uint64)
+      requires ValidDstAddr64(mem, id, addr);
+      ensures id in mem;
+      ensures mem[id].Heaplet64?;
+      ensures addr in mem[id].mem64;
+{
+}
+
+lemma lemma_ValidSrcAddr64(mem:Heaplets, id:heaplet_id, addr : uint64, t:taint)
+      requires ValidSrcAddr64(mem, id, addr, t); 
+      ensures id in mem;
+      ensures mem[id].Heaplet64?;
+      ensures addr in mem[id].mem64;
+      ensures addr in mem[id].mem64;
+      ensures mem[id].mem64[addr].t == t;
+      ensures ValidDstAddr64(mem, id, addr);
+{
+}
+
+predicate Mem64ChangedOnlyAtWith(mem: Heaplets, old_mem : Heaplets, id : heaplet_id, 
+             addr : uint64, off : uint64, value : uint64, t : taint)
+    requires ValidSrcAddr64(old_mem, id, addr + off, Public); 
+{
+  mem == old_mem[id := old_mem[id].(mem64 := old_mem[id].mem64[addr + off := Heaplet64Entry(value, t)])]
+} 
 
 }
