src/crypto/loopunroll/addrlogic.s.dfy
@@ -1,0 +1,215 @@
+include "../../lib/util/types.s.dfy"
+include "../../lib/util/operations.s.dfy"
+include "../../lib/util/words_and_bytes.s.dfy"
+include "../../lib/collections/Seqs.s.dfy"
+include "../../arch/x64/def.s.dfy"
+include "../../arch/x64/vale.i.dfy"
+include "../../lib/util/dafny_wrappers.i.dfy"
+
+module addrlogic {
+
+import opened x64_def_s
+import opened types_s
+import opened x64_vale_i
+import opened dafny_wrappers_i
+
+// Unaligned 
+predicate ValidDstUnAddr64(h:Heaplets, id:heaplet_id, addr:int)
+{
+  id in h  && 
+  h[id].Heaplet64? && 
+  addr in h[id].mem64
+}
+
+predicate ValidSrcUnAddr64(h:Heaplets, id:heaplet_id, addr:int, taint:taint) 
+{
+  id in h  && 
+  h[id].Heaplet64? && 
+  addr in h[id].mem64 &&
+  h[id].mem64[addr].t == taint
+}
+
+lemma lemma_ValidDstUnAddr64(mem:Heaplets, id:heaplet_id, addr : uint64)
+      requires ValidDstUnAddr64(mem, id, addr);
+      ensures id in mem;
+      ensures mem[id].Heaplet64?;
+      ensures addr in mem[id].mem64;
+{
+}
+
+lemma lemma_ValidSrcUnAddr64(mem:Heaplets, id:heaplet_id, addr : uint64, t:taint)
+      requires ValidSrcUnAddr64(mem, id, addr, t); 
+      ensures id in mem;
+      ensures mem[id].Heaplet64?;
+      ensures addr in mem[id].mem64;
+      ensures mem[id].mem64[addr].t == t;
+      ensures ValidDstUnAddr64(mem, id, addr);
+{
+}
+
+predicate ValidDstUnAddrs64(mem:Heaplets, id:heaplet_id, addr:int, count : nat)
+ requires count > 0;
+ requires addr + (count - 1) * 8 < 0x1_0000_0000_0000_0000;
+{
+  id in mem &&
+  mem[id].Heaplet64? &&
+  forall i: nat :: 0 < i <= count  ==> addr + (i - 1) * 8 in mem[id].mem64 &&
+  forall i : nat :: 0 < i <= count ==> ValidDstUnAddr64(mem, id, addr + (i - 1) * 8)
+}
+
+predicate ValidSrcUnAddrs64(mem:Heaplets, id:heaplet_id, addr:int, taint:taint, count : nat) 
+ requires count > 0;
+ requires addr + (count - 1) * 8 < 0x1_0000_0000_0000_0000;
+{
+  id in mem &&
+  mem[id].Heaplet64? &&
+  forall i: nat :: 0 < i <= count  ==> addr + (i - 1) * 8 in mem[id].mem64 &&
+  forall i : nat :: 0 < i <= count ==> ValidSrcUnAddr64(mem, id, addr + (i - 1) * 8, taint)
+}
+
+lemma lemma_ValidDstUnAddrs64(mem:Heaplets, id:heaplet_id, addr : uint64, count : nat)
+      requires count > 0;
+      requires addr + (count - 1) * 8 < 0x1_0000_0000_0000_0000;
+      requires ValidDstUnAddrs64(mem, id, addr, count);
+      ensures id in mem;
+      ensures mem[id].Heaplet64?;
+      ensures forall i : nat :: 0 < i <= count ==> addr + (i - 1) * 8  in mem[id].mem64;
+      ensures forall i : nat :: 0 < i <= count ==> ValidDstUnAddr64(mem, id, addr + (i - 1) * 8);
+{}
+
+lemma lemma_ValidSrcUnAddrs64(mem:Heaplets, id:heaplet_id, addr : uint64, taint : taint, count : int)
+      requires count > 0;
+      requires addr + (count - 1) * 8 < 0x1_0000_0000_0000_0000;
+      requires ValidSrcUnAddrs64(mem, id, addr, taint, count);
+      ensures id in mem;
+      ensures mem[id].Heaplet64?;
+      ensures forall i : nat :: 0 < i <= count ==> addr + (i - 1) * 8  in mem[id].mem64;
+      ensures forall i: nat ::  0 < i < count ==> ValidSrcUnAddr64(mem, id, addr + (i - 1) * 8, taint);
+      ensures forall i : nat :: 0 < i <= count ==> ValidDstUnAddr64(mem, id, addr + (i - 1) * 8);
+      ensures ValidDstUnAddrs64(mem, id, addr, count);
+{}
+
+// Aligned
+
+predicate ValidDstAlAddr64(h:Heaplets, id:heaplet_id, addr:int)
+{
+  id in h  && 
+  h[id].Heaplet64? && 
+  addr in h[id].mem64 &&
+  addr % 8 == 0
+}
+
+predicate ValidSrcAlAddr64(h:Heaplets, id:heaplet_id, addr:int, taint:taint) 
+{
+  id in h  && 
+  h[id].Heaplet64? && 
+  addr in h[id].mem64 &&
+  h[id].mem64[addr].t == taint &&
+  addr % 8 == 0
+}
+
+lemma lemma_ValidDstAlAddr64(mem:Heaplets, id:heaplet_id, addr : uint64)
+      requires ValidDstAlAddr64(mem, id, addr);
+      ensures id in mem;
+      ensures mem[id].Heaplet64?;
+      ensures addr in mem[id].mem64;
+      ensures addr % 8 == 0;
+      ensures ValidDstUnAddr64(mem, id, addr);
+{
+}
+
+lemma lemma_ValidSrcAlAddr64(mem:Heaplets, id:heaplet_id, addr : uint64, t:taint)
+      requires ValidSrcAlAddr64(mem, id, addr, t); 
+      ensures id in mem;
+      ensures mem[id].Heaplet64?;
+      ensures addr in mem[id].mem64;
+      ensures addr % 8 == 0;
+      ensures mem[id].mem64[addr].t == t;
+      ensures ValidSrcUnAddr64(mem, id, addr, t); 
+      ensures ValidDstAlAddr64(mem, id, addr);
+      ensures ValidDstUnAddr64(mem, id, addr);
+{
+}
+
+predicate ValidDstAlAddrs64(mem:Heaplets, id:heaplet_id, addr:int, count : nat)
+ requires count > 0;
+ requires addr + (count - 1) * 8 < 0x1_0000_0000_0000_0000;
+{
+  id in mem &&
+  mem[id].Heaplet64? &&
+  addr % 8 == 0 &&
+  forall i : nat :: 0 < i <= count ==> (addr + (i - 1) * 8) % 8 == 0 &&
+  forall i : nat :: 0 < i <= count ==> addr + (i - 1) * 8 in mem[id].mem64 &&
+  forall i : nat :: 0 < i <= count ==> ValidDstAlAddr64(mem, id, addr + (i - 1) * 8)
+}
+
+predicate ValidSrcAlAddrs64(mem:Heaplets, id:heaplet_id, addr:int, taint:taint, count : nat) 
+ requires count > 0;
+ requires addr + (count - 1) * 8 < 0x1_0000_0000_0000_0000;
+{
+  id in mem &&
+  mem[id].Heaplet64? &&
+  addr % 8 == 0 &&
+  forall i : nat :: 0 < i <= count ==> (addr + (i - 1) * 8) % 8 == 0 &&
+  forall i : nat :: 0 < i <= count ==> addr + (i - 1) * 8 in mem[id].mem64 &&
+  forall i : nat :: 0 < i <= count ==> ValidSrcAlAddr64(mem, id, addr + (i - 1) * 8, taint) &&
+  forall i : nat :: 0 < i <= count ==> 
+   (ValidSrcAlAddr64(mem, id, addr + (i - 1) * 8, taint) ==>
+   mem[id].mem64[addr + (i - 1) * 8].t == taint)
+}
+
+lemma lemma_ValidDstAlAddrs64(mem:Heaplets, id:heaplet_id, addr : uint64, count : nat)
+      requires count > 0;
+      requires addr + (count - 1) * 8 < 0x1_0000_0000_0000_0000;
+      requires ValidDstAlAddrs64(mem, id, addr, count);
+      ensures id in mem;
+      ensures mem[id].Heaplet64?;
+      ensures forall i : nat :: 0 < i <= count ==> addr + (i - 1) * 8  in mem[id].mem64;
+      ensures forall i : nat :: 0 < i <= count ==> ValidDstAlAddr64(mem, id, addr + (i - 1) * 8);
+      ensures forall i : nat :: 0 < i <= count ==> ValidDstUnAddr64(mem, id, addr + (i - 1) * 8);
+{}
+
+lemma lemma_ValidSrcAlAddrs64(mem:Heaplets, id:heaplet_id, addr : uint64, taint : taint, count : int)
+      requires count > 0;
+      requires addr + (count - 1) * 8 < 0x1_0000_0000_0000_0000;
+      requires ValidSrcAlAddrs64(mem, id, addr, taint, count);
+      ensures id in mem;
+      ensures mem[id].Heaplet64?;
+      ensures ValidDstAlAddrs64(mem, id, addr, count);
+      ensures ValidDstUnAddrs64(mem, id, addr, count);
+      ensures forall i : nat :: 0 < i <= count ==> addr + (i - 1) * 8  in mem[id].mem64;
+      ensures forall i : nat :: 0 < i <= count ==> ValidSrcAlAddr64(mem, id, addr + (i - 1) * 8, taint);
+      ensures forall i : nat :: 0 < i <= count ==> ValidSrcUnAddr64(mem, id, addr + (i - 1) * 8, taint);
+      ensures forall i : nat :: 0 < i <= count ==> 
+                (ValidSrcAlAddr64(mem, id, addr + (i - 1) * 8, taint) ==>
+                 mem[id].mem64[addr + (i - 1) * 8].t == taint)
+      ensures forall i : nat :: 0 < i <= count ==> ValidDstAlAddr64(mem, id, addr + (i - 1) * 8);
+{
+}
+
+// OnlyUpdates
+
+
+predicate OnlyUpdatesAddr64(old_mem : Heaplets, mem : Heaplets, id:heaplet_id, addr : uint64, taint:taint, v:uint64)
+    requires ValidDstUnAddr64(old_mem, id, addr);
+{
+  mem == old_mem[id := old_mem[id].(mem64 := old_mem[id].mem64[addr := Heaplet64Entry(v, taint)])]
+}
+
+predicate RestUntouched64(old_mem : Heaplets, mem : Heaplets, id:heaplet_id, addr : uint64) 
+  requires ValidDstUnAddr64(old_mem, id, addr);
+{  
+  // I don't delelete any heaplet.
+  (forall nid : heaplet_id :: nid in old_mem ==> nid in mem) && 
+  // I don't modify any other heaplet.
+  (forall nid : heaplet_id :: nid in old_mem && nid != id ==> nid in mem && mem[nid] == old_mem[nid]) &&
+  // mem[id] is still a Healplet64
+  id in mem && mem[id].Heaplet64? &&
+  // I only adjusted this one address in old_mem[id].
+  (forall naddr : uint64 :: naddr != addr && naddr in old_mem[id].mem64 ==> 
+    naddr in mem[id].mem64 && mem[id].mem64[naddr] == old_mem[id].mem64[naddr])
+}
+
+
+
+}
